IGrammarSafety.v
@@ -1,0 +1,180 @@
+Require Export IGrammar.
+Require Import MyUtils.
+
+Section IGrammarSafety.
+
+Arguments ANode {_ _} _.
+Arguments INode {_ _} _ _ _.
+
+Arguments HPatt {_}.
+Arguments IPatt {_} _ _ _.
+
+Arguments prio {_} _ _ _.
+Arguments left_a {_} _ _ _.
+Arguments right_a {_} _ _ _.
+
+Lemma dec_conflict_pattern {O} (pr : drules O) `{drules_dec pr} (q : tree_pattern O) :
+  Decision (conflict_pattern pr q).
+Proof.
+  destruct drules_dec0.
+  unfold Decision. destruct q.
+  - right. intro. inv H.
+  - destruct q1, q2.
+    + right. intro. inv H.
+    + destruct q2_1. destruct q2_2.
+      * replace (IPatt HPatt o (IPatt HPatt o0 HPatt)) with (CR o o0); try reflexivity.
+        specialize dec_prio with (o1 := o) (o2 := o0).
+        specialize dec_left_a with (o1 := o) (o2 := o0).
+        destruct dec_prio, dec_left_a; auto using CPrio2, CLeft.
+        right. intro. inv H; contradiction.
+      * right. intro. inv H.
+      * right. intro. inv H.
+    + destruct q1_1. destruct q1_2.
+      * replace (IPatt (IPatt HPatt o0 HPatt) o HPatt) with (CL o o0); try reflexivity.
+        specialize dec_prio with (o1 := o) (o2 := o0).
+        specialize dec_right_a with (o1 := o) (o2 := o0).
+        destruct dec_prio, dec_right_a; auto using CPrio1, CRight.
+        right. intro. inv H; contradiction.
+      * right. intro. inv H.
+      * right. intro. inv H.
+    + right. intro. inv H.
+Qed.
+
+Lemma safe_cl_cr {O} (o1 o2 : O) (pr : drules O) `{safety_props pr} :
+  (conflict_pattern pr (CL o1 o2) /\ conflict_pattern pr (CR o2 o1)) -> False.
+Proof.
+  intros H_CL_CR. destruct safety_props0.
+  destruct H_CL_CR as [H_CL H_CR].
+  inv H_CL; inv H_CR.
+  - apply prio_antisym in H0. contradiction.
+  - apply left_a_sym in H1.
+    apply prio_one in H0. destruct H0. contradiction.
+  - apply right_a_sym in H0.
+    apply prio_one in H1. destruct H1. contradiction.
+  - apply right_a_sym in H0.
+    apply left_a_one in H1. destruct H1. contradiction.
+Qed.
+
+Lemma linsert_one_match {L O} (pr : drules O) (l : L) (o1 : O) (t t' : parse_tree L O) :
+  linsert_one pr l o1 t t' ->
+  matches t' (IPatt HPatt o1 HPatt) \/
+  (exists o2 : O, matches t (IPatt HPatt o2 HPatt) /\ matches t' (IPatt HPatt o2 HPatt)).
+Proof.
+  intros. inv H.
+  - left. apply IMatch; apply HMatch.
+  - left. apply IMatch; apply HMatch.
+  - right. exists o2. split; apply IMatch; apply HMatch.
+Qed.
+
+Lemma conflict_pattern_cases {O} (pr : drules O) (q : tree_pattern O) (P : Prop) :
+  (forall o1 o2, q = CL o1 o2 -> P) ->
+  (forall o1 o2, q = CR o1 o2 -> P) ->
+  (conflict_pattern pr q -> P).
+Proof.
+  intros. inv H1; eauto.
+Qed.
+
+Lemma linsert_one_safe {L O} (pr : drules O) `{safety_props pr}
+    (l1 : L) (o1 : O) (t t' : parse_tree L O) :
+  conflict_free (conflict_pattern pr) t ->
+  linsert_one pr l1 o1 t t' ->
+  conflict_free (conflict_pattern pr) t'.
+Proof.
+  intros. induction H0.
+  - apply INode_cfree; auto using ANode_cfree.
+    intro. inv H0. inv H1. inv H0; inv H2.
+    inv H4. inv H9. inv H9. inv H4.
+  - apply INode_cfree; auto using ANode_cfree.
+    intro. inv H1. inv H2. 
+    eapply conflict_pattern_cases; try eassumption; intros; subst; inv H3.
+    + inv H5.
+    + inv H10. eauto using safe_cl_cr.
+  - inv H. apply INode_cfree; auto.
+    intro. inv H. inv H2.
+    eapply conflict_pattern_cases; try eassumption; intros; subst; inv H3.
+    + apply linsert_one_match in H1. destruct H1.
+      * inv H1. inv H8. eauto using safe_cl_cr.
+      * inv H1. inv H2. inv H8. inv H3. inv H1.
+        apply H5. exists (CL o0 x). split; try assumption.
+        unfold CL. auto using HMatch, IMatch.
+    + inv H13. apply H5.
+      exists (CR o0 o3). split; try assumption.
+      unfold CR. auto using HMatch, IMatch.
+Qed.
+
+Lemma linsert_one_yield {L O} (pr : drules O)
+    (l1 : L) (o1 : O) (t t' : parse_tree L O) :
+  linsert_one pr l1 o1 t t' ->
+  yield t' = inl l1 :: inr o1 :: yield t .
+Proof.
+  intros. induction H; simpl; auto.
+  rewrite IHlinsert_one. reflexivity.
+Qed.
+
+Lemma linsert_one_exists {L O} (pr : drules O) `{drules_dec pr}
+    (l : L) (o : O) (t : parse_tree L O) :
+  exists t', linsert_one pr l o t t'.
+Proof.
+  induction t.
+  - eexists. apply ANode_LInsert_One.
+  - assert (Decision (conflict_pattern pr (CR o o0))). {
+      auto using dec_conflict_pattern.
+    }
+    destruct IHt1, IHt2.
+    destruct H.
+    + eexists. eauto using INode_LInsert_One_2.
+    + eexists. eauto using INode_LInsert_One_1.
+Qed.
+
+Lemma linsert_yield {L O} (pr : drules O)
+    (o : O) (t1 t2 t' : parse_tree L O) :
+  linsert pr t1 o t2 t' ->
+  yield t' = yield t1 ++ inr o :: yield t2.
+Proof.
+  intro. induction H; simpl; eauto using linsert_one_yield.
+  - rewrite IHlinsert2. rewrite IHlinsert1.
+    simplify_list_eq. reflexivity.
+Qed.
+
+Lemma linsert_safe {L O} (pr : drules O) `{safety_props pr}
+    (o : O) (t1 t2 t' : parse_tree L O) :
+  conflict_free (conflict_pattern pr) t2 ->
+  linsert pr t1 o t2 t' ->
+  conflict_free (conflict_pattern pr) t'.
+Proof.
+  intros. induction H0; eauto using linsert_one_safe.
+Qed.
+
+Lemma linsert_exists {L O} (pr : drules O) `{drules_dec pr}
+    (o : O) (t1 t2 : parse_tree L O) :
+  exists t', linsert pr t1 o t2 t'.
+Proof.
+  revert o t2. induction t1; intros.
+  - assert (exists t', linsert_one pr l o t2 t'). {
+      auto using linsert_one_exists.
+    }
+    destruct H. eauto using ANode_LInsert.
+  - specialize IHt1_2 with o0 t2. destruct IHt1_2.
+    specialize IHt1_1 with o x. destruct IHt1_1.
+    eauto using INode_LInsert.
+Qed.
+
+Theorem safety {L O} (pr : drules O) `{safety_props pr} `{drules_dec pr} (w : list (L + O)) :
+  language w -> dlanguage pr w.
+Proof.
+  unfold language, dlanguage. intro. destruct H as [t].
+  revert H. revert w. induction t; intros; simpl in *.
+  - exists (ANode l); simpl in *. split.
+    + assumption.
+    + apply ANode_cfree.
+  - specialize IHt2 with (yield t2). destruct IHt2 as [t2']. reflexivity. destruct H0.
+    assert (exists t', linsert pr t1 o t2' t'). {
+      auto using linsert_exists.
+    }
+    destruct H2 as [t']. exists t'. split.
+    + rewrite <- H. rewrite <- H0.
+      eauto using linsert_yield.
+    + eauto using linsert_safe.
+Qed.
+
+End IGrammarSafety.
